more sorting

Weidenbach_Book/WB_Sort.thy
@@ -4,72 +4,126 @@ theory WB_Sort
 begin
 
 definition partition_between :: \<open>('b \<Rightarrow> 'b \<Rightarrow> bool) \<Rightarrow> ('a \<Rightarrow> 'b) \<Rightarrow> nat \<Rightarrow> nat \<Rightarrow> 'a list \<Rightarrow> ('a list \<times> nat) nres\<close> where
-  \<open>partition_between R h i j xs = do {
-     ASSERT(i \<le> length xs \<and> j \<le> length xs);
-     pivot \<leftarrow> RETURN (h (xs ! i));
-     (i, j, xs) \<leftarrow> WHILE\<^sub>T\<^bsup> \<lambda>(i, j, xs'). mset xs' = mset xs\<^esup> 
-       (\<lambda>(i, j, xs). i < j)
-       (\<lambda>(i, j, xs). do {
-          i \<leftarrow> WHILE\<^sub>T(\<lambda>i. R (h (xs ! i)) pivot \<and> i < j)
-            (\<lambda>i. RETURN (i+1))
-	    i;
-          j \<leftarrow> WHILE\<^sub>T(\<lambda>j. R pivot (h (xs ! j)) \<and> j > i)
-                (\<lambda>j. RETURN (j-1))
-	        j;
-	  let xs = (if (i < j) then swap xs i j else xs);
-	  RETURN (i, j, xs)
+  \<open>partition_between R h i0 j0 xs0 = do {
+     ASSERT(i0 < length xs0 \<and> j0 < length xs0);
+     pivot \<leftarrow> RETURN (h (xs0 ! j0));
+     (i, xs) \<leftarrow> FOREACHi
+       (\<lambda>js (i, xs). i < length xs \<and> mset xs = mset xs0 \<and> i \<ge> i0 \<and>
+          i \<le> (j0 - 1) - card js)
+       (set [i0..<j0 - 1])
+       (\<lambda>j (i, xs). do {
+         ASSERT(j < length xs);
+         if R (h (xs!j)) pivot
+	 then RETURN (i+1, swap xs i j)
+	 else RETURN (i, xs)
        })
-       (i,j, xs);
-     RETURN (xs, j)
+       (i0, xs0);
+     RETURN (xs, i+1)
    }\<close>
 
+lemma Min_atLeastLessThan[simp]: \<open>b > a \<Longrightarrow> Min {a..<b} = a\<close> for a b :: nat
+  using linorder_class.eq_Min_iff[of \<open>{a..<b}\<close> a]
+  by (auto simp: )
+
+lemma Min_atLeastLessThan2[simp]: \<open>{a..<b} \<noteq> {} \<Longrightarrow> Min {a..<b} = a\<close> for a b :: nat
+  using linorder_class.eq_Min_iff[of \<open>{a..<b}\<close> a]
+  by (auto simp: )
+
+
+lemma partition_between_mset_eq:
+  assumes \<open>i < length xs\<close> and \<open>j < length xs\<close> and \<open>j > i\<close>
+  shows \<open>partition_between R h i j xs \<le> SPEC(\<lambda>(xs', j'). mset xs = mset xs' \<and> j' < length xs \<and>
+     j' > i \<and> j' \<le> j)\<close>
+proof -
+  show ?thesis
+    unfolding partition_between_def
+    apply (refine_vcg WHILEIT_rule[where R = \<open>measure (\<lambda>(i, j, _). j - i)\<close>])
+    subgoal using assms by auto
+    subgoal using assms by auto
+    subgoal by auto
+    subgoal using assms by auto
+    subgoal using assms by auto
+    subgoal by auto
+    subgoal using assms by (auto dest: mset_eq_length)
+    subgoal by (force dest: mset_eq_length)
+    subgoal by (force dest: mset_eq_length)
+    subgoal by auto
+    subgoal by auto
+    subgoal for x it \<sigma> a b x1 x2
+      apply (subst card_Diff_singleton)
+      apply (auto dest: finite_subset simp: card_gt_0_iff)
+apply (subst Suc_pred)
+apply (auto dest: finite_subset simp: card_gt_0_iff)
+by (smt One_nat_def Suc_diff_Suc Suc_diff_le Suc_le_mono Suc_pred \<open>i < length xs \<and> j < length xs \<Longrightarrow> finite (set [i..<j - 1])\<close> assms(3) card_atLeastLessThan card_mono diff_Suc_Suc less_le nat_in_between_eq(2) neq0_conv set_upt zero_less_diff)
+    subgoal by auto
+    subgoal by auto
+    subgoal by auto
+    subgoal for x it \<sigma> a b x1 x2
+      by (subst card_Diff_singleton)
+        (auto dest: finite_subset simp: card_gt_0_iff)
+    subgoal by auto
+    subgoal using assms by auto
+    subgoal by auto
+    subgoal using assms(3) by auto
+    done
+qed
 
 definition quicksort :: \<open>_ \<Rightarrow> _ \<Rightarrow> nat \<Rightarrow> nat \<Rightarrow> 'a::ord list \<Rightarrow> 'a list nres\<close> where
 \<open>quicksort R h i j xs0 = do {
   RECT (\<lambda>f (i,j,xs). do {
       ASSERT(mset xs = mset xs0);
-      if i \<ge> j then RETURN xs
+      if i+1 \<ge> j then RETURN xs
       else do{
 	(xs, k) \<leftarrow> partition_between R h i j xs;
-	xs \<leftarrow> f (i, k, xs);
-	f (k+1, j, xs)
+	xs \<leftarrow> f (i, k-1, xs);
+	f (k, j, xs)
       }
     })
     (i, j, xs0)
   }\<close>
 
-lemma "quicksort (<) id 0 5 [12, (0::nat), (5::nat), (1::nat), 2, 6] = A"
+
+lemma quicksort_between_mset_eq:
+  assumes \<open>i < length xs\<close> and \<open>j < length xs\<close> and \<open>j \<ge> i\<close>
+  shows \<open>quicksort R h i j xs \<le> \<Down> Id (SPEC(\<lambda>xs'. mset xs = mset xs'))\<close>
 proof -
-				      
+  have wf: \<open>wf (measure (\<lambda>(i, j, xs). Suc j - i))\<close>
+    by auto
+  have pre: \<open>(\<lambda>(i, j, xs'). i < length xs \<and> j < length xs \<and> i \<le> j \<and>
+    mset xs = mset xs') (i,j,xs)\<close>
+    using assms by auto
   show ?thesis
-    supply WHILET_unfold[simp] WHILEIT_unfold[simp] 
-    unfolding quicksort_def partition_between_def
-    apply (simp add: quicksort_def partition_between_def RECT_unfold)
-    apply (subst RECT_unfold, refine_mono, simp add: WHILEIT_unfold)
-    apply (subst RECT_unfold, refine_mono)
-    apply (simp add: )
-    apply (subst RECT_unfold, refine_mono)
-    apply (simp add: WHILEIT_unfold)
-    apply (subst RECT_unfold, refine_mono)
-    apply (simp add: WHILEIT_unfold)
-    apply (subst RECT_unfold, refine_mono)
-    apply (simp add: WHILEIT_unfold)
-    apply (subst RECT_unfold, refine_mono)
-    apply (simp add: WHILEIT_unfold)
-    apply (subst RECT_unfold, refine_mono)
-    apply (simp add: WHILET_unfold)
-    apply (subst RECT_unfold, refine_mono)
-    apply (simp add: WHILET_unfold)
-    apply (subst RECT_unfold, refine_mono)
-    apply (simp add: WHILET_unfold)
-    apply (subst RECT_unfold, refine_mono)
-    apply (simp add: WHILET_unfold)
-    apply (subst RECT_unfold, refine_mono)
-    apply (simp add: WHILET_unfold)
-    apply (subst RECT_unfold, refine_mono)
-    apply (simp add: WHILET_unfold)
-    apply (subst RECT_unfold, refine_mono)
-    apply (simp add: WHILET_unfold)
-    apply (simp add: swap_def)
-  oops
+    unfolding quicksort_def
+    apply (rule RECT_rule)
+       apply (refine_mono)
+      apply (rule wf)
+     apply (rule pre)
+    subgoal premises IH for f x
+      using IH(2)
+      apply (refine_vcg)
+      apply ((auto; fail)+)[2]
+      apply (rule partition_between_mset_eq[THEN order_trans])
+      subgoal by (auto dest: mset_eq_length)
+      subgoal by (auto dest: mset_eq_length)
+      subgoal by (auto dest: mset_eq_length)
+      apply (rule SPEC_rule)
+      apply (subst (5) Down_id_eq[symmetric])
+      apply (case_tac xa, simp only: prod.simps)
+      apply (rule bind_refine_spec)
+      prefer 2
+      apply (rule IH(1)[THEN order_trans])
+      subgoal
+        by (auto dest: mset_eq_length)
+      subgoal by auto
+      apply (subst (3) Down_id_eq[symmetric])
+      apply (rule order.refl)
+      apply (rule IH(1)[THEN order_trans])
+      subgoal
+        by (auto dest: mset_eq_length)
+      subgoal by auto
+      apply auto
+      done
+    done
+qed
+
 end
